lean/Brainfuck.lean
@@ -10,6 +10,8 @@ import Brainfuck.Program.RawProgram
 import Brainfuck.Program.Validate
 import Brainfuck.Program.ValidatedProgram
 import Brainfuck.Proofs.Cell
+import Brainfuck.Proofs.Eval
+import Brainfuck.Proofs.Pointer
 import Brainfuck.Proofs.Step
 import Brainfuck.Semantics.Eval
 import Brainfuck.Semantics.Step
