lean/Brainfuck/Core/Result.lean
@@ -3,7 +3,7 @@ namespace Brainfuck.Core
 inductive Result (α ε : Type) where
   | ok : α → Result α ε
   | err : ε → Result α ε
-  deriving Repr
+  deriving DecidableEq, Repr
 
 namespace Result
 
@@ -15,6 +15,17 @@ def bind {α β ε : Type} (value : Result α ε) (f : α → Result β ε) : Re
   match value with
   | .ok okValue => f okValue
   | .err error => .err error
+
+instance {ε : Type} : Functor (fun α => Result α ε) where
+  map := map
+
+instance {ε : Type} : Pure (fun α => Result α ε) where
+  pure := Result.ok
+
+instance {ε : Type} : Bind (fun α => Result α ε) where
+  bind := bind
+
+instance {ε : Type} : Monad (fun α => Result α ε) where
 
 end Result
 
